compiling coq code for timestamp and event

example/event.go
@@ -7,20 +7,20 @@ import (
 
 type Event struct {
 	id    uint32
-	start *TimeStamp
-	end   *TimeStamp
+	startTime *TimeStamp
+	endTime   *TimeStamp
 }
 
 func (e *Event) approxSize() uint64 {
-	size := std.SumAssumeNoOverflow(4, e.start.approxSize())
-	return std.SumAssumeNoOverflow(size, e.end.approxSize())
+	size := std.SumAssumeNoOverflow(4, e.startTime.approxSize())
+	return std.SumAssumeNoOverflow(size, e.endTime.approxSize())
 }
 
 func MarshalEvent(e *Event, prefix []byte) []byte {
 	var enc = prefix
 	enc = marshal.WriteInt32(enc, e.id)
-	enc = MarshalTimeStamp(e.start, enc)
-	enc = MarshalTimeStamp(e.end, enc)
+	enc = MarshalTimeStamp(e.startTime, enc)
+	enc = MarshalTimeStamp(e.endTime, enc)
 	return enc
 }
 
@@ -28,7 +28,7 @@ func UnmarshalEvent(s []byte) (*Event, []byte) {
 	e := new(Event)
 	var enc = s // Needed for goose compatibility
 	e.id, enc = marshal.ReadInt32(enc)
-	e.start, enc = UnmarshalTimeStamp(enc)
-	e.end, enc = UnmarshalTimeStamp(enc)
+	e.startTime, enc = UnmarshalTimeStamp(enc)
+	e.endTime, enc = UnmarshalTimeStamp(enc)
 	return e, enc
 }
