example/grackle_Event_proof.v
@@ -1,35 +1,39 @@
 From Perennial.program_proof Require Import grove_prelude.
 From Grackle.example Require Import example.
 From Perennial.program_proof Require Import marshal_stateless_proof.
-From Grackle.example Require Import timestamp_proof.
+From Grackle.example Require Import grackle_TimeStamp_proof.
 
 Module Event.
 Section Event.
 
+Typeclasses Opaque app.
+
 Context `{!heapGS Σ}.
 
 Record C :=
-  mkC {
-      id : u32 ;
-      startTime : TimeStamp.C ;
-      endTime : TimeStamp.C ;
-    }.
+    mkC {
+        id : u32;
+        startTime : TimeStamp.C;
+        endTime : TimeStamp.C;
+        }.
 
 Definition has_encoding (encoded:list u8) (args:C) : Prop :=
-  ∃ start_enc end_enc,
-  encoded = (u32_le args.(id)) ++ start_enc ++ end_enc
-  /\ TimeStamp.has_encoding start_enc args.(startTime)
-  /\ TimeStamp.has_encoding end_enc args.(endTime).
+  ∃ (startTime_enc endTime_enc : list u8), 
+  encoded = (u32_le args.(id)) ++
+              startTime_enc ++
+              endTime_enc
+  /\ TimeStamp.has_encoding startTime_enc args.(startTime)
+  /\ TimeStamp.has_encoding endTime_enc args.(endTime).
 
-Definition own args_ptr args q : iProp Σ :=
-  ∃ (start_l end_l: loc),
+Definition own (args_ptr:loc) (args:C) (q:dfrac) : iProp Σ :=
+  ∃ (startTime_l endTime_l : loc),
   "Hargs_id" ∷ args_ptr ↦[Event :: "id"]{q} #args.(id) ∗
-  "Hargs_start" ∷ args_ptr ↦[Event :: "startTime"]{q} #start_l ∗
-  "Hargs_start_enc" ∷ TimeStamp.own start_l args.(startTime) q ∗
-  "Hargs_end" ∷ args_ptr ↦[Event :: "endTime"]{q} #end_l ∗
-  "Hargs_end_enc" ∷ TimeStamp.own end_l args.(endTime) q.
+  "Hargs_startTime" ∷ args_ptr ↦[Event :: "startTime"]{q} #startTime_l ∗
+  "Hargs_startTime_enc" ∷ TimeStamp.own startTime_l args.(startTime) q ∗
+  "Hargs_endTime" ∷ args_ptr ↦[Event :: "endTime"]{q} #endTime_l ∗
+  "Hargs_endTime_enc" ∷ TimeStamp.own endTime_l args.(endTime) q.
 
-Lemma wp_Encode (args_ptr:loc) (args:C) (prefix:list u8) (pre_sl:Slice.t) :
+Lemma wp_Encode (args_ptr:loc) (args:C) (pre_sl:Slice.t) (prefix:list u8) :
   {{{
         own args_ptr args (DfracDiscarded) ∗
         own_slice pre_sl byteT (DfracOwn 1) prefix
@@ -40,35 +44,34 @@ Lemma wp_Encode (args_ptr:loc) (args:C) (prefix:list u8) (pre_sl:Slice.t) :
         ⌜has_encoding enc args⌝ ∗
         own_slice enc_sl byteT (DfracOwn 1) (prefix ++ enc)
   }}}.
+
 Proof.
   iIntros (?) "H HΦ". iDestruct "H" as "[Hown Hsl]". iNamed "Hown".
   wp_rec. wp_pures.
   wp_apply (wp_ref_to); first by val_ty.
   iIntros (?) "Hptr". wp_pures.
-
   wp_loadField. wp_load. wp_apply (wp_WriteInt32 with "[$Hsl]").
   iIntros (?) "Hsl". wp_store.
 
   wp_load. wp_loadField.
-  wp_apply (TimeStamp.wp_Encode with "[$Hargs_start_enc $Hsl]").
-  iIntros (start_enc start_sl) "Hsl".
+  wp_apply (TimeStamp.wp_Encode with "[$Hargs_startTime_enc $Hsl]").
+  iIntros (startTime_enc startTime_sl) "Hsl".
   iDestruct "Hsl" as (Hencoding_startTime) "Hsl". wp_store.
 
   wp_load. wp_loadField.
-  wp_apply (TimeStamp.wp_Encode with "[$Hargs_end_enc $Hsl]").
-  iIntros (end_enc end_sl) "Hsl".
+  wp_apply (TimeStamp.wp_Encode with "[$Hargs_endTime_enc $Hsl]").
+  iIntros (endTime_enc endTime_sl) "Hsl".
   iDestruct "Hsl" as (Hencoding_endTime) "Hsl". wp_store.
 
   wp_load. iApply "HΦ". iModIntro. rewrite -?app_assoc.
   iFrame. iPureIntro.
 
-  unfold has_encoding. exists start_enc, end_enc. split. { exact. }
+  unfold has_encoding. exists startTime_enc, endTime_enc. 
+  split. { exact. }
   split. { exact. } { exact. }
 Qed.
 
-Typeclasses Opaque app.
-
-Lemma wp_Decode enc enc_sl (args:C) (suffix : list u8) (q : dfrac) :
+Lemma wp_Decode enc enc_sl (args:C) (suffix:list u8) (q:dfrac):
   {{{
         ⌜has_encoding enc args⌝ ∗
         own_slice_small enc_sl byteT q (enc ++ suffix)
@@ -78,28 +81,28 @@ Lemma wp_Decode enc enc_sl (args:C) (suffix : list u8) (q : dfrac) :
         args_ptr suff_sl, RET (#args_ptr, suff_sl); own args_ptr args (DfracOwn 1) ∗
                                                     own_slice_small suff_sl byteT q suffix
   }}}.
+
 Proof.
   iIntros (?) "[%Henc Hsl] HΦ". wp_rec.
   wp_apply wp_allocStruct; first by val_ty.
-  iIntros (?) "Hs". wp_pures.
+  iIntros (?) "Hstruct". wp_pures.
   wp_apply wp_ref_to; first done.
   iIntros (?) "Hptr". wp_pures.
-  iDestruct (struct_fields_split with "Hs") as "HH".
+  iDestruct (struct_fields_split with "Hstruct") as "HH".
   iNamed "HH".
 
   unfold has_encoding in Henc.
-  destruct Henc as (startTime_sl & endTime_sl & Henc & Hencoding_startTime & Hencoding_endTime).
+  destruct Henc as ( startTime_sl & endTime_sl & Henc & Hencoding_startTime & Hencoding_endTime ).
   rewrite Henc. rewrite -?app_assoc.
 
   wp_load. wp_apply (wp_ReadInt32 with "[$Hsl]"). iIntros (?) "Hsl".
   wp_pures. wp_storeField. wp_store.
 
-  wp_load.
-  wp_apply (TimeStamp.wp_Decode startTime_sl with "[Hsl]").
+  wp_load. wp_apply (TimeStamp.wp_Decode startTime_sl with "[Hsl]").
   { iFrame. exact. } iIntros (??) "[HstartTime Hsl]". wp_pures. wp_storeField. wp_store.
 
-  wp_load.
-  wp_apply (TimeStamp.wp_Decode endTime_sl with "[Hsl]").
+
+  wp_load. wp_apply (TimeStamp.wp_Decode endTime_sl with "[Hsl]").
   { iFrame. exact. } iIntros (??) "[HendTime Hsl]". wp_pures. wp_storeField. wp_store.
 
   wp_load. wp_pures. iApply "HΦ". iModIntro. iFrame.
@@ -107,3 +110,4 @@ Qed.
 
 End Event.
 End Event.
+
