example/grackle_TimeStamp_proof.v
@@ -2,24 +2,26 @@ From Perennial.program_proof Require Import grove_prelude.
 From Grackle.example Require Import example.
 From Perennial.program_proof Require Import marshal_stateless_proof.
 
-(* Annotations and discussion for this file is in timestamp_proof.org *)
-
 Module TimeStamp.
 Section TimeStamp.
+
+Typeclasses Opaque app.
 
 Context `{!heapGS Σ}.
 
 Record C :=
-  mkC {
-      hour : u32 ;
-      minute : u32 ;
-      second : u32 ;
-    }.
+    mkC {
+        hour : u32;
+        minute : u32;
+        second : u32;
+        }.
 
 Definition has_encoding (encoded:list u8) (args:C) : Prop :=
-  encoded = (u32_le args.(hour)) ++ (u32_le args.(minute)) ++ (u32_le args.(second)).
+  encoded = (u32_le args.(hour)) ++
+              (u32_le args.(minute)) ++
+              (u32_le args.(second)).
 
-Definition own args_ptr args q : iProp Σ :=
+Definition own (args_ptr:loc) (args:C) (q:dfrac) : iProp Σ :=
   "Hargs_hour" ∷ args_ptr ↦[TimeStamp :: "hour"]{q} #args.(hour) ∗
   "Hargs_minute" ∷ args_ptr ↦[TimeStamp :: "minute"]{q} #args.(minute) ∗
   "Hargs_second" ∷ args_ptr ↦[TimeStamp :: "second"]{q} #args.(second).
@@ -40,23 +42,21 @@ Proof.
   iIntros (?) "H HΦ". iDestruct "H" as "[Hown Hsl]". iNamed "Hown".
   wp_rec. wp_pures.
   wp_apply (wp_ref_to); first by val_ty.
-  iIntros (?) "Hptr".
-  wp_pures.
-
+  iIntros (?) "Hptr". wp_pures.
+  wp_loadField. wp_load. wp_apply (wp_WriteInt32 with "[$Hsl]").
+  iIntros (?) "Hsl". wp_store.
+  wp_loadField. wp_load. wp_apply (wp_WriteInt32 with "[$Hsl]").
+  iIntros (?) "Hsl". wp_store.
   wp_loadField. wp_load. wp_apply (wp_WriteInt32 with "[$Hsl]").
   iIntros (?) "Hsl". wp_store.
 
-  wp_loadField. wp_load. wp_apply (wp_WriteInt32 with "[$Hsl]").
-  iIntros (?) "Hsl". wp_store.
+  wp_load. iApply "HΦ". iModIntro. rewrite -?app_assoc.
+  iFrame. iPureIntro.
 
-  wp_loadField. wp_load. wp_apply (wp_WriteInt32 with "[$Hsl]").
-  iIntros (?) "Hsl". wp_store.
-
-  wp_load. iApply "HΦ". iModIntro. rewrite -?app_assoc. iFrame.
-  iPureIntro. done.
+   done.
 Qed.
 
-Lemma wp_Decode enc enc_sl (args:C) (suffix : list u8) (q : dfrac):
+Lemma wp_Decode enc enc_sl (args:C) (suffix:list u8) (q:dfrac):
   {{{
         ⌜has_encoding enc args⌝ ∗
         own_slice_small enc_sl byteT q (enc ++ suffix)
@@ -70,23 +70,25 @@ Lemma wp_Decode enc enc_sl (args:C) (suffix : list u8) (q : dfrac):
 Proof.
   iIntros (?) "[%Henc Hsl] HΦ". wp_rec.
   wp_apply wp_allocStruct; first by val_ty.
-  iIntros (?) "Hs". wp_pures.
+  iIntros (?) "Hstruct". wp_pures.
   wp_apply wp_ref_to; first done.
   iIntros (?) "Hptr". wp_pures.
-  iDestruct (struct_fields_split with "Hs") as "HH".
-  iNamed "HH". rewrite Henc.
+  iDestruct (struct_fields_split with "Hstruct") as "HH".
+  iNamed "HH".
 
-  wp_load. wp_apply (wp_ReadInt32 with "[$]"). iIntros (?) "Hs".
+  rewrite Henc. rewrite -?app_assoc.
+
+  wp_load. wp_apply (wp_ReadInt32 with "[$Hsl]"). iIntros (?) "Hsl".
   wp_pures. wp_storeField. wp_store.
 
-  wp_load. wp_apply (wp_ReadInt32 with "[$]"). iIntros (?) "Hs".
+  wp_load. wp_apply (wp_ReadInt32 with "[$Hsl]"). iIntros (?) "Hsl".
   wp_pures. wp_storeField. wp_store.
 
-  wp_load. wp_apply (wp_ReadInt32 with "[$]"). iIntros (?) "Hs".
+  wp_load. wp_apply (wp_ReadInt32 with "[$Hsl]"). iIntros (?) "Hsl".
   wp_pures. wp_storeField. wp_store.
-
   wp_load. wp_pures. iApply "HΦ". iModIntro. iFrame.
 Qed.
 
 End TimeStamp.
 End TimeStamp.
+
